---
tags:
  - math-493
aliases:
  - the derived subgroup
  - derived subgroup
  - the commutator subgroup
  - The Commutator Subgroup
  - commutator subgroup
---
Relevant Classes: [[Math 493]]

> [!info] **Definition: The Derived Subgroup**
> 
> Let $G$ be a group. The derived subgroup $[G,G]$ of $G$ is the subgroup generated by its commutators: $$ [G,G] = \langle x y x^{-1} y^{-1} \mid x, y \in G \rangle. $$

This subgroup has a few interesting and useful properties.

> [!example] **Normality**
> 
> Fix an element in $[G, G]$. It is of the form $x y x^{-1} y ^{-1}$. Thus, we have:
> 
> $$\begin{align*}  (xyx^{-1}y^{-1})g^{-1} &= gxg^{-1} gyg^{-1} gx^{-1}g^{-1} gy^{-1}g^{-1} \\  &= (gxg^{-1}) (gyg^{-1}) (gxg^{-1})^{-1} (gyg^{-1})^{-1}  \end{align*}$$
 > 
 > which is another commutator, and thus is in $[G, G]$.

Since $[G, G] \triangleleft G$, we can take the quotient group $G / [G, G]$. This has a few interesting properties:

1. $G/[G, G]$ is abelian.
2. If $G/N$ is abelian, then $[G, G] \subseteq N$. Thus, $G/[G, G]$ is the largest abelian quotient group.

> [!example] **Abelian**
> 
> Fix two cosets, $x [G, G]$ and $y[G, G]$. We want to show that 
> $$ (x[G, G]) (y[G, G]) = (y[G, G]) (x[G, G]). $$ 
> 
> $$ \begin{align*} 
> (x[G, G]) (y[G, G]) &= x y [G, G] \\
> &= xy (y^{-1} x^{-1} y x [G, G]) \\
> &= y x [G, G] \\
> &= (y[G, G]) (x[G, G]).
> \end{align*} $$
> 
> Thus, $G/[G, G]$ is abelian.


> [!example] **Largest Abelian Subgroup**
> 
> Suppose $N$ is a normal subgroup of $G$ and $G/N$ is abelian. Then, we have $(xN)(yN) = (yN)(xN)$ which means that $xyN = yxN$, which gives us that $$ y^{-1}x^{-1} y x N = N \implies  y^{-1}x^{-1} y x \in N. $$
> 
> That means that the derived subgroup $[G, G] \leq N$.
> 
